Specify + Prove X64.Vale.InsMem

vale/code/arch/x64/X64.Stack_i.fst
@@ -6,3 +6,6 @@ let valid_src_stack64 i st = admit()
 let valid_dst_stack64 i st = admit()
 let load_stack64 i st = admit()
 let store_stack64 i v h = admit()
+let free_stack64 start finish h = admit()
+
+let init_rsp h = admit()
