vale/code/arch/x64/X64.Stack_Sems.fst
@@ -2,3 +2,23 @@ module X64.Stack_Sems
 
 let stack_to_s s = admit()
 let stack_from_s s = admit()
+
+let lemma_state_of_to s = admit()
+
+let equiv_valid_src_stack64 ptr h = admit()
+
+let equiv_valid_dst_stack64 rsp ptr h = admit()
+
+let equiv_load_stack64 ptr h = admit()
+
+let free_stack_same_load start finish ptr h =
+  let S.Vale_stack _ mem = h in
+  let S.Vale_stack _ mem' = S.free_stack' start finish h in
+  Classical.forall_intro (Vale.Set.remove_between_reveal (Map.domain mem) start finish);
+  Opaque_s.reveal_opaque S.get_heap_val64_def
+
+let equiv_store_stack64 ptr v h = admit()
+
+let store64_same_init_rsp ptr v h = admit()
+
+let equiv_free_stack start finish h = admit()
