vale/code/arch/x64/X64.Stack_i.fsti
@@ -5,6 +5,9 @@ open X64.Machine_s
 val stack: Type u#1
 
 val valid_src_stack64 : ptr:int -> h:stack -> GTot bool
-val valid_dst_stack64 : ptr:int -> h:stack -> GTot bool
+val valid_dst_stack64 : rsp:int -> ptr:int -> h:stack -> GTot bool
 val load_stack64 : ptr:int -> h:stack -> GTot nat64
 val store_stack64 : ptr:int -> v:nat64 -> h:stack -> GTot stack
+val free_stack64 : start:int -> finish:int -> h:stack -> GTot stack
+
+val init_rsp: h:stack -> nat64
